src/fourbitcounter_OK.v
@@ -11,10 +11,68 @@ Require Import fourbitcount2.
 
 Set Implicit Arguments.
 
+Definition ruleMap0 (_: RegsT): string -> option string :=
+  "increment" |-> "increment"; "done" |-> "done"; ||.
+Definition ruleMap1 (_: RegsT): string -> option string :=
+  "increment" |-> "increment"; "done" |-> "done"; ||.
+
+Definition regMap (r: RegsT): RegsT.
+  (* We are using tactics to build a map from register valuations in [impl] to register valuations in [spec]. *)
+  kgetv "c.top"%string datav r (Bit 4) (M.empty _: RegsT).
+  (* First, extract the value of [impl] register ["data"]. *)
+  exact (M.add "c.top"%string (existT _ _ datav) (M.empty _)).
+  (* Then, give the corresponding values of all registers for [spec]. *)
+Defined.
+Hint Unfold ruleMap0: MethDefs.
+Hint Unfold ruleMap1: MethDefs.
+Hint Unfold regMap: MethDefs. (* for kdecompose_regMap_init *)
+
+Theorem fourbitcounter_0_OK :
+   fourbitcount2.module'mkTb.mkTb "top" <<== fourbitcount2.module'spec.spec0 "top".
+Proof.
+    kinline_compute.
+    kdecompose_nodefs regMap ruleMap0.
+    kinvert.
+    kinv_magic.
+    * destruct wlt_dec. trivial. contradiction.
+    * kinv_magic.
+Qed.
+
+Theorem fourbitcounter_1_OK :
+   fourbitcount2.module'mkTb.mkTb "top" <<== fourbitcount2.module'spec.spec1 "top".
+Proof.
+    kinline_compute.
+    kdecompose_nodefs regMap ruleMap1.
+    kinvert.
+    kinv_magic.
+    * trivial.  kinv_magic.
+   destruct wlt_dec. trivial. contradiction.
+    * kinv_magic.
+Qed.
+
+Definition ruleMap (_: RegsT): string -> option string :=
+  "increment" |-> "spec_rule"; "done" |-> "spec_rule"; ||.
+Hint Unfold ruleMap: MethDefs.
+Hint Unfold regMap: MethDefs. (* for kdecompose_regMap_init *)
+
 Theorem fourbitcounter_OK :
-   fourbitcount2.spec.spec "top" <<== fourbitcount2.module'mkTb.mkTb "top".
+   fourbitcount2.module'mkTb.mkTb "top" <<== fourbitcount2.module'spec.spec "top".
 
 Proof.
+kinline_compute.
+kdecompose_nodefs regMap ruleMap.
+kinv_magic.
 admit. (* fixme: proof goes here *)
 
 Admitted.
+
+Theorem fourbitcounter_2_OK :
+   fourbitcount2.module'spec.spec2 "top" <<== fourbitcount2.module'spec.spec2 "top".
+
+Proof.
+kinline_compute.
+kdecompose_nodefs regMap ruleMap1.
+kinv_magic.
+admit. (* fixme proof *)
+Admitted.
+
